cleanup

examples/wysteria/examples/attic/psitestiface.fsi
@@ -1,0 +1,11 @@
+(*--build-config
+    options:--admit_fsi FStar.Set --admit_fsi Wysteria --admit_fsi FStar.OrdSet --admit_fsi FStar.IO --admit_fsi Smciface;
+    other-files:ghost.fst ext.fst set.fsi heap.fst st.fst all.fst io.fsti list.fst listTot.fst st2.fst ordset.fsi ../../prins.fst ../ffi.fst ../wysteria.fsi psitest.fst
+ --*)
+
+module Smciface
+
+open Prins
+open FStar.OrdSet
+
+val psi: ps:prins{ps = union (singleton Alice) (singleton Bob)} -> p:prin{mem p ps} -> x:list int -> Tot (list int)
