examples/wysteria/ml/hashtable.ml
@@ -1,0 +1,12 @@
+module Hashtbl = Extlib.ExtHashtbl.Hashtbl
+
+type ('a, 'b) t = ('a, 'b) Hashtbl.t
+
+let create n = Hashtbl.create n
+
+let find t k = Hashtbl.find t k
+
+let mem t k = Hashtbl.mem t k
+
+let add t k v =
+  Hashtbl.add t k v; t
