examples/wysteria/theory.fst
@@ -221,7 +221,8 @@ val slice_concat_lemma_sps:
           (ensures (slice_tr_sps ps (concat_traces tr1 tr2) = concat_traces (slice_tr_sps ps tr1) (slice_tr_sps ps tr2)))
     [SMTPat (slice_tr_sps ps (concat_traces tr1 tr2))]
 let slice_concat_lemma_sps ps tr1 tr2 = admit()
-(* CH: this fails on my laptop with Unknown assertion failed
+(* CH: this times out on my laptop with Unknown assertion failed
+   AR: works for me
   slice_h_append_lemma_forall_sps ();
   let _ = assert (slice_tr_sps_h ps (append (reveal tr1) (reveal tr2)) = append (slice_tr_sps_h ps (reveal tr1)) (slice_tr_sps_h ps (reveal tr2))) in
   ()
@@ -793,6 +794,7 @@ val slice_concat_lemma:
     [SMTPat (slice_tr p (concat_traces tr1 tr2))]
 let slice_concat_lemma p tr1 tr2 = admit()
 (* CH: this fails on my laptop with Unknown assertion failed
+   AR: works for me
   slice_h_append_lemma_forall ();
   let _ = assert (slice_tr_h p (append (reveal tr1) (reveal tr2)) = append (slice_tr_h p (reveal tr1)) (slice_tr_h p (reveal tr2))) in
   ()
